move sim.sml to a lib

gol_simLib.sig
@@ -1,0 +1,28 @@
+signature gol_simLib =
+sig
+
+datatype bexp = False
+              | True
+              | Var of string * int
+              | Not of bexp
+              | And of bexp * bexp
+              | Or of bexp * bexp;
+
+datatype dir = N | S | W | E;
+
+type io_port = (int * int) * dir;
+
+type gate =
+  { filename : string ,
+    inputs : io_port list ,
+    outputs : io_port list ,
+    height : int ,
+    width : int };
+
+type state
+
+val load: gate -> state
+
+val run_to_fixpoint: state -> bexp vector vector
+
+end;
