gol_rulesScript.sml
@@ -2275,22 +2275,4 @@ Proof
   \\ metis_tac [ALL_DISTINCT_MAP_FST,PAIR_EQ]
 QED
 
-(* --- examples --- *)
-
-Definition set_env_def:
-  set_env a b (A,n:num) = (a n):bool ∧
-  set_env a b (B,n:num) = (b n):bool
-End
-
-Theorem wire_e_e_sim[local]: (* fake *)
-  simulation_ok 1 1 [((-1,0),E,Var A 5)] [((1,0),E,Var A 0)] [ (* ... *) ]
-Proof
-  cheat
-QED
-
-Theorem wire_e_e_raw =
-  MATCH_MP simulation_ok_IMP_circuit wire_e_e_sim
-  |> Q.SPEC ‘set_env a b’
-  |> SRULE [eval_io_def,EVAL “make_area 1 1”, set_env_def, SF ETA_ss];
-
 val _ = export_theory();
