gol_exampleScript.sml
@@ -1,0 +1,23 @@
+open bossLib gol_rulesTheory;
+
+val _ = new_theory "gol_example";
+
+(* --- examples --- *)
+
+Definition set_env_def:
+  set_env a b (A,n:num) = (a n):bool ∧
+  set_env a b (B,n:num) = (b n):bool
+End
+
+Theorem wire_e_e_sim[local]: (* fake *)
+  simulation_ok 1 1 [((-1,0),E,Var A 5)] [((1,0),E,Var A 0)] [ (* ... *) ]
+Proof
+  cheat
+QED
+
+Theorem wire_e_e_raw =
+  MATCH_MP simulation_ok_IMP_circuit wire_e_e_sim
+  |> Q.SPEC ‘set_env a b’
+  |> SRULE [eval_io_def,EVAL “make_area 1 1”, set_env_def, SF ETA_ss];
+
+val _ = export_theory();
